\documentclass[12pt,a4paper,fleqn]{article}
\usepackage[utf8]{inputenc}
\usepackage{amssymb, amsmath, multicol}
\usepackage[russian]{babel}
\usepackage{graphicx}
\graphicspath{{pictures/}}
\DeclareGraphicsExtensions{.pdf,.png,.jpg}
\usepackage[shortcuts,cyremdash]{extdash}
\usepackage{wrapfig}
\usepackage{floatflt}
\usepackage{lipsum}
\usepackage{concmath}
\usepackage{euler}
\usepackage{tikz}  
\usetikzlibrary{graphs}

\oddsidemargin=-15.4mm
\textwidth=190mm
\headheight=-32.4mm
\textheight=277mm
\tolerance=100
\parindent=0pt
\parskip=8pt
\pagestyle{empty}
\renewcommand{\tg}{\mathop{\mathrm{tg}}\nolimits}
\renewcommand{\ctg}{\mathop{\mathrm{ctg}}\nolimits}
\renewcommand{\arctan}{\mathop{\mathrm{arctg}}\nolimits}
\newcommand{\divisible}{\mathop{\raisebox{-2pt}{\vdots}}}

\begin{document}
{\bf 1a)} $1 + x + x^2 + \ldots + x^n = \dfrac{x^{n + 1} - 1}{x - 1}$ \newline
$x \cdot (1 + x + x^2 + \ldots + x^n)' = x + 2x^2 + \ldots + nx^n \rightarrow$ \newline
$x + 2x^2 + \ldots + nx^n = x \cdot \left(\dfrac{x^{n + 1} - 1}{x - 1} \right)' = \dfrac{nx^{n + 2} - (n + 1)x^{n + 1} + x}{(x - 1)^2}$ \newline
$x \cdot (x + 2x^2 + \ldots + nx^n)' = x + 2^2x^2 + 3^2x^3 + \ldots + n^2x^n = \sum_{k = 1}^n k^2x^k$ (искомая сумма, где $x = \dfrac{1}{4}$) $\rightarrow$ \newline
$\sum_{k = 1}^n k^2x^k = x \cdot (\dfrac{nx^{n + 2} - (n + 1)x^{n + 1} + x}{(x - 1)^2})' = \dfrac{n^2x^{n + 3} + (-2n^2 - 2n + 1)x^{n + 2} + (n^2 + 2n + 1)x^{n + 1} - x^2 - x}{(x - 1)^3}$ \newline \newline
{\bf 1c)} $\sum_{k=0}^\infty x^k = \dfrac{1}{1 - x} (|x| < 1) \rightarrow$ \newline
$\dfrac{1}{x} \int \sum_{k=0}^\infty x^k = \dfrac{1}{x} \sum_{k=0}^\infty \dfrac{x^{k + 1}}{k + 1} = \sum_{k = 0}^n \dfrac{x^k}{k + 1}$ \newline
$\dfrac{1}{x} \int \sum_{k=0}^\infty x^k = \dfrac{1}{x} \int \dfrac{1}{1 - x} = -\ln (1 -x) \dfrac{1}{x} = -\dfrac{\ln (1 - x)}{x}$ \newline \newline
{\bf 1d)} $(- \cos (kx))' = k \cdot \sin (kx)$ \newline
$\sum_{k=0}^n \cos (kx) = \dfrac{\cos (nx + \frac{x}{2})}{2\cos\frac{x}{2}} - \dfrac{1}{2}$ (см. 2d) $\rightarrow$ \newline
$\sum_{k=0}^n k \cdot \sin (kx) = - (\dfrac{\cos (nx + \frac{x}{2})}{2\cos\frac{x}{2}} - \dfrac{1}{2})' = \dfrac{\cos (nx + \frac{x}{2}) \cdot \sin \frac{x}{2} - \sin (nx + \frac{x}{2}) \cdot (n + \frac{1}{2}) \cdot \cos \frac{x}{2}}{2 \cos^2 \frac{x}{2}}$ \newline \newline
{\bf 1f)} $\sum_{k=0}^n \dfrac{5^{2k}}{3^{4n-3k}} C_n^k = \dfrac{1}{81^n} \sum_{k=0}^n 25^k \cdot 27^k \cdot C_n^k = \dfrac{1}{81^n} \sum_{k=0}^n 675^k C_n^k = \dfrac{(1 + 675)^n}{81^n} = \left( \dfrac{676}{81} \right) ^n$ \newline \newline
{\bf 2a)} $k \equiv 1\mod 2 \rightarrow$ \newline
$a_k = \dfrac{-k}{4k^2 - 1} = -\dfrac{1}{4(2k - 1)} - \dfrac{1}{4(2k + 1)}$ \newline
$a_{k + 1} = \dfrac{1}{4(2k + 1)} + \dfrac{1}{4(2k + 3)}$ \newline
$a_{k + 2} = - \dfrac{1}{4(2k + 3)} - \dfrac{1}{4(2k + 5)}$ \newline
$a_{k + 3} = \dfrac{1}{4(2k + 5)} + \dfrac{1}{4(2k + 7)} \rightarrow$ \newline
$\sum_{k = 1}^n \dfrac{(-1)^k \cdot k}{4k^2 - 1} = \dfrac{(-1)^n \cdot n}{4(2n + 1)} -\dfrac{1}{12}$ \newline \newline
{\bf 2b)} $[x]_k = x(x-2)(x-4)\ldots(x - 2(k - 1)) \rightarrow$ \newline
$[x + 2]_{k + 1} - [x]_{k + 1} = (x+2)x(x-2) \ldots (x - 2(k-1)) - x(x-2)\ldots (x - 2(k -1))(x - 2k) = (x + 2 - x + 2k)x(x-2)\ldots(x-2(k-1)) = (2k + 2)[x]_k \rightarrow$ \newline
$[x]_k = \dfrac{[x+2]_{k + 1} - [x]_{k + 1}}{2n + 2} \rightarrow$ \newline
$\sum_{x=1}^n [x]_k = \dfrac{1}{2k + 2} \sum_{x = 1}^n [x+2]_{k+1} - [x]_{k+1} = \dfrac{1}{2n + 2} ([n+2]_{k+1} + [n+1]_{k+1} - [2]_{k+1} - [1]_{k+1})$ \newline \newline
{\bf 2d)} $\cos(kx) = \dfrac{2\cdot \cos (kx) \cdot \cos \frac{x}{2}}{2 \cdot \cos \frac{x}{2}} = \dfrac{\cos (kx + \frac{x}{2}) - \cos (kx - \frac{x}{2})}{2 \cdot \cos \frac{x}{2}} \rightarrow$ \newline
$\sum_{k = 0}^n \cos (kx) = \dfrac{1}{2\cos \frac{x}{2}} \sum_{k=0}^n(\cos (kx + \frac{x}{2}) - \cos (kx - \frac{x}{2})) = \dfrac{1}{2\cos\frac{x}{2}} (\cos (nx + \frac{x}{2})- \cos \frac{x}{2}) = \dfrac{\cos (nx + \frac{x}{2})}{2\cos\frac{x}{2}} - \dfrac{1}{2}$ \newline \newline
{\bf 3e)} $(1 + i)^{4m} = \sum_{k = 0}^{4m} C_{4m}^k i^k$ \newline
$k \equiv 0 \mod 4 \rightarrow C_{4m}^k i^k = C_{4m}^k$ \newline
$k \equiv 1 \mod 4 \rightarrow C_{4m}^k i^k = C_{4m}^k i$ \newline
$k \equiv 2 \mod 4 \rightarrow C_{4m}^k i^k = -C_{4m}^k$ \newline
$k \equiv 3 \mod 4 \rightarrow C_{4m}^k i^k = -C_{4m}^k i$ \newline
$\rightarrow$ Если $k \equiv 1 (3) \mod 4$, то $(4m - k) \equiv 3(1) \mod 4 \rightarrow C_{4m}^k i^k + C_{4m - k}^k i^{4m - k} = 0 \rightarrow$ \newline
$(1 + i)^{4m} = C_{4m}^0 - C_{4m}^2 + \ldots + C_{4m}^{4m}$ \newline \newline
{\bf 3f)} $i(1 + i)^{4m} = \sum_{k = 0}^{4m} C_{4m}^k i^{k + 1}$ \newline
$k \equiv 0 \mod 4 \rightarrow C_{4m}^k i^{k + 1} = C_{4m}^k i$ \newline
$k \equiv 1 \mod 4 \rightarrow C_{4m}^k i^{k + 1} = - C_{4m}^k$ \newline
$k \equiv 2 \mod 4 \rightarrow C_{4m}^k i^{k + 1} = - C_{4m}^k i$ \newline
$k \equiv 3 \mod 4 \rightarrow C_{4m}^k i^{k + 1} = C_{4m}^k$ \newline
$\rightarrow k \equiv 0(2) \mod 4 \rightarrow (4m - k) \equiv 2(0) \mod 4 \rightarrow C_{4m}^k i^{k + 1} + C_{4m}^{4m - k} i^{4m - k + 1} = 0$ \newline
$i(1 + i)^{4m} = - C_{4m}^1 + C_{4m}^3 + \ldots + C_{4m}^{4m - 1} \rightarrow$ \newline
$C_{4m}^1 - C_{4m}^3 + \ldots - C_{4m}^{4m - 1} = -i(1 + i)^{4m}$
 \end{document}